Set interface and implementation with rbt, remdups adapted

Example_Automatic.thy
@@ -2,17 +2,7 @@ theory Example_Automatic
   imports "Refine_Imperative_HOL/Sepref" "SepLogicTime_RBTreeBasic.RBTree_Impl"
     Set_Impl2  
 begin
- 
 
-lemma set_init_hnr'_short[sepref_fr_rules]:
-  "hn_refine (emp) set_empty emp rbt_set_assn (set_init_SPEC)"
-  sorry
-
-lemma set_ins_hnr_abs[sepref_fr_rules]:
-  "hn_refine (hn_ctxt rbt_set_assn S p * hn_val Id x x')
-       (rbt_set_insert x' p)
-       (hn_invalid rbt_set_assn S p * hn_val Id x x') rbt_set_assn (set_ins_SPEC $ x $ S)"
-  sorry
 
 (*
 lemma set_mem_hnr_abs[sepref_fr_rules]:
@@ -20,23 +10,11 @@ lemma set_mem_hnr_abs[sepref_fr_rules]:
      (rbt_search (x'::nat) p)
      (hn_ctxt rbt_set_assn S p * hn_val Id x x') Y' ( (set_mem_SPEC $ x $ S))"
   sorry *)
-
-definition rbt_mem :: "nat \<Rightarrow> (nat, unit) rbt_node ref option \<Rightarrow> bool Heap" where 
-  "rbt_mem x p = do {
-      f \<leftarrow> rbt_search x p;
-      ureturn (f = Some ()) }"
-
-lemma set_mem_hnr [sepref_fr_rules]:
-  "hn_refine (hn_ctxt rbt_set_assn S p * hn_val Id x x')
-     (rbt_mem (x'::nat) p)
-     (hn_ctxt rbt_set_assn S p * hn_val Id x x') id_assn ( (set_mem_SPEC $ x $ S))"
-  sorry
-
-
+ 
 definition rd_impl1 :: "nat list \<Rightarrow> (nat list) nrest" where
   "rd_impl1 as = do {
           ys \<leftarrow> RETURNT [];
-          S \<leftarrow> set_init_SPEC;
+          S \<leftarrow> mop_empty_set 1;
           zs \<leftarrow> RETURNT as;
           (zs,ys,S) \<leftarrow> whileT (\<lambda>(xs,ys,S). length xs > 0)
             (\<lambda>(xs,ys,S). do {                          
@@ -45,10 +23,10 @@ definition rd_impl1 :: "nat list \<Rightarrow> (nat list) nrest" where
                           ASSERT (card S \<le> length ys);
                           x \<leftarrow> RETURNT (hd xs);
                           xs \<leftarrow> RETURNT (tl xs);
-                          b \<leftarrow> set_mem_SPEC x S;
+                          b \<leftarrow> mop_mem_set (\<lambda>S. rbt_search_time_logN (length as + 1) + 1) x S;
                           (if b
   then  RETURNT (xs,ys,S)
-  else do { S \<leftarrow> set_ins_SPEC x S;
+  else do { S \<leftarrow> mop_insert_set (\<lambda>S. rbt_insert_logN (length as + 1)) x S;
             ys \<leftarrow> RETURNT (x#ys);  
             RETURNT (xs,ys,S)
   } ) }) (zs,ys,S);
@@ -89,15 +67,31 @@ lemma hn_refine_tl[sepref_fr_rules]: " hn_refine (hn_val Id s' s)
        (pure Id) (RETURNT $ (tl $ s'))"
   unfolding hn_refine_def apply (auto simp:   mult.assoc  execute_ureturn pure_def hn_ctxt_def)
      by (auto simp: top_assn_rule zero_enat_def relH_def  elim: pureD )      
- 
 
-(* synthesize *)
+
+
+
+(* synthesize *) 
 
 context 
   fixes as::"nat list"
   notes [[sepref_register_adhoc as]]
   notes [sepref_import_param] = IdI[of as] 
 begin
+
+declare rbt_search_time_logN_mono [intro]
+declare rbt_insert_logN_mono [intro]
+
+sepref_definition test is "uncurry0 (rd_impl1 as)" :: "unit_assn\<^sup>k \<rightarrow>\<^sub>a list_assn nat_assn"
+  unfolding rd_impl1_def
+  apply sepref 
+  done
+print_theorems
+term test
+thm test_def 
+thm test.refine[to_hnr] 
+
+(*
 
 schematic_goal synth_rd: "hn_refine emp (?C::?'a Heap) ?\<Gamma>' ?R (rd_impl1 as)" using [[goals_limit = 3]]
   unfolding rd_impl1_def
@@ -118,12 +112,14 @@ schematic_goal synth_rd: "hn_refine emp (?C::?'a Heap) ?\<Gamma>' ?R (rd_impl1 a
   apply sepref_dbg_constraints
   done
 
- 
+thm synth_rd[to_hfref]
+
+
 concrete_definition rd_impl uses synth_rd is "hn_refine _ (?c ) _ _ _"
 
 thm rd_impl_def
 term rd_impl
-
+*)
 end
 
 
